WebAssembly/Wasm_Printing/Wasm_Type_Abs_Printing.thy
@@ -138,6 +138,10 @@ code_printing
 | constant si32_trunc_f32 \<rightharpoonup> (OCaml) "I32Wrapper'_convert.trunc'_s'_f32"
 | constant ui64_trunc_f32 \<rightharpoonup> (OCaml) "I64Wrapper'_convert.trunc'_u'_f32"
 | constant si64_trunc_f32 \<rightharpoonup> (OCaml) "I64Wrapper'_convert.trunc'_s'_f32"
+| constant ui32_trunc_sat_f32 \<rightharpoonup> (OCaml) "I32Wrapper'_convert.trunc'_u'_f32"
+| constant si32_trunc_sat_f32 \<rightharpoonup> (OCaml) "I32Wrapper'_convert.trunc'_s'_f32"
+| constant ui64_trunc_sat_f32 \<rightharpoonup> (OCaml) "I64Wrapper'_convert.trunc'_u'_f32"
+| constant si64_trunc_sat_f32 \<rightharpoonup> (OCaml) "I64Wrapper'_convert.trunc'_s'_f32"
 (* FLOAT64 *)
   (* UNOPS *)
 | constant wasm_float_f64_inst.float_neg_f64 \<rightharpoonup> (OCaml) "F64Wrapper.neg"
@@ -167,6 +171,10 @@ code_printing
 | constant si32_trunc_f64 \<rightharpoonup> (OCaml) "I32Wrapper'_convert.trunc'_s'_f64"
 | constant ui64_trunc_f64 \<rightharpoonup> (OCaml) "I64Wrapper'_convert.trunc'_u'_f64"
 | constant si64_trunc_f64 \<rightharpoonup> (OCaml) "I64Wrapper'_convert.trunc'_s'_f64"
+| constant ui32_trunc_sat_f64 \<rightharpoonup> (OCaml) "I32Wrapper'_convert.trunc'_u'_f64"
+| constant si32_trunc_sat_f64 \<rightharpoonup> (OCaml) "I32Wrapper'_convert.trunc'_s'_f64"
+| constant ui64_trunc_sat_f64 \<rightharpoonup> (OCaml) "I64Wrapper'_convert.trunc'_u'_f64"
+| constant si64_trunc_sat_f64 \<rightharpoonup> (OCaml) "I64Wrapper'_convert.trunc'_s'_f64"
 
 code_printing
   constant serialise_i32 \<rightharpoonup> (OCaml) "ImplWrapper.serialise_i32"
