WebAssembly/Wasm_Properties.thy
@@ -14,6 +14,16 @@ lemma t_cvt: assumes "cvt t sx v = Some v'" shows "t = typeof v'"
   apply (simp add: option.case_eq_if, metis option.discI option.inject v.simps(20))
   done
 
+lemma t_cvt_sat: assumes "cvt_sat t sx v = Some v'" shows "t = typeof v'"
+  using assms
+  unfolding cvt_sat_def typeof_def
+  apply (cases t)
+      apply (simp add: option.case_eq_if, metis option.discI option.inject v.simps(17))
+    apply (simp add: option.case_eq_if, metis option.discI option.inject v.simps(18))
+   apply (simp add: option.case_eq_if, metis option.discI option.inject v.simps(19))
+  apply (simp add: option.case_eq_if, metis option.discI option.inject v.simps(20))
+  done
+
 lemma store_preserved1:
   assumes "\<lparr>s;vs;es\<rparr> \<leadsto>_i \<lparr>s';vs';es'\<rparr>"
           "store_typing s \<S>"
@@ -217,6 +227,7 @@ lemma typeof_cvtop:
           "e = Cvtop t1 cvtop t sx"
   shows "(typeof v) = t"
         "cvtop = Convert \<Longrightarrow> (t1 \<noteq> t) \<and> ((sx = None) = ((is_float_t t1 \<and> is_float_t t) \<or> (is_int_t t1 \<and> is_int_t t \<and> (t_length t1 < t_length t))))"
+        "cvtop = ConvertSat \<Longrightarrow> (t1 \<noteq> t) \<and> (sx = None) = ((is_float_t t1 \<and> is_float_t t) \<or> (is_int_t t1 \<and> is_int_t t \<and> (t_length t1 < t_length t)))"
         "cvtop = Reinterpret \<Longrightarrow> (t1 \<noteq> t) \<and> t_length t1 = t_length t"
 proof -
   have  "\<C> \<turnstile> [C v, e] : (ts _> ts')"
@@ -227,6 +238,7 @@ proof -
     by fastforce
   show "(typeof v) = t"
        "cvtop = Convert \<Longrightarrow> (t1 \<noteq> t) \<and> (sx = None) = ((is_float_t t1 \<and> is_float_t t) \<or> (is_int_t t1 \<and> is_int_t t \<and> (t_length t1 < t_length t)))"
+       "cvtop = ConvertSat \<Longrightarrow> (t1 \<noteq> t) \<and> (sx = None) = ((is_float_t t1 \<and> is_float_t t) \<or> (is_int_t t1 \<and> is_int_t t \<and> (t_length t1 < t_length t)))"
        "cvtop = Reinterpret \<Longrightarrow> (t1 \<noteq> t) \<and> t_length t1 = t_length t"
     using b_e_type_value[OF ts''_def(1)] b_e_type_cvtop[OF ts''_def(2) assms(2)]
     by simp_all
@@ -252,7 +264,7 @@ proof -
   have "arity_1_result e = typeof (v')"
     using assms(1,3)
     apply (cases rule: reduce_simple.cases)
-             apply (simp_all add: arity_1_result_def wasm_deserialise_type t_cvt)
+             apply (simp_all add: arity_1_result_def wasm_deserialise_type t_cvt t_cvt_sat)
            apply (auto simp add: typeof_def)
     done
   hence "\<C> \<turnstile> [C v'] : ([] _> [arity_1_result e])"
@@ -1154,6 +1166,16 @@ next
     by simp
 next
   case (convert_None t1 v t2 sx)
+  then show ?thesis
+    using e_typing_s_typing.intros(4)
+    by simp
+next
+  case (convert_sat_Some t1 v t2 sx v')
+  then show ?thesis
+    using assms(1, 3) types_preserved_unop_testop_cvtop
+    by simp
+next
+  case (convert_sat_None t1 v t2 sx)
   then show ?thesis
     using e_typing_s_typing.intros(4)
     by simp
@@ -2443,6 +2465,25 @@ next
     case (Some a)
     thus ?thesis
       using reduce.intros(1)[OF reduce_simple.convert_Some[OF _ Some]] cs_def
+      unfolding types_agree_def
+      by fastforce
+  qed
+next
+  case (convert_sat t1 t2 sx \<C>)
+  obtain v where cs_def:"cs = [$ C v]" "typeof v = t2"
+    using const_typeof const_of_const_list[OF _ convert_sat(6)] e_type_const_list[OF convert_sat(6,3)]
+    by fastforce
+  thus ?case
+  proof (cases "cvt_sat t1 sx v")
+    case None
+    thus ?thesis
+      using reduce.intros(1)[OF reduce_simple.convert_sat_None[OF _ None]] cs_def
+      unfolding types_agree_def
+      by fastforce
+  next
+    case (Some a)
+    thus ?thesis
+      using reduce.intros(1)[OF reduce_simple.convert_sat_Some[OF _ Some]] cs_def
       unfolding types_agree_def
       by fastforce
   qed
